TM/LM/HeapTM.v
@@ -2,7 +2,9 @@ Require Export TM.Code.CodeTM TM.Code.Copy.
 Require Export TM.Code.MatchNat TM.Code.MatchSum TM.Code.MatchFin TM.Code.MatchPair TM.Code.WriteValue.
 Require Export TM.Code.ChangeAlphabet TM.LiftMN TM.LiftSigmaTau.
 Require Export TM.Basic.Mono.
+(*
 Require Export TM.Code.ListTM. (* [Nth] *)
+*)
 Require Export TM.LM.Definitions TM.LM.TokTM.
 
 
@@ -12,27 +14,36 @@ Require Export TM.LM.Definitions TM.LM.TokTM.
 (** ** Alphabets *)
 
 (* See [TokTM] *)
+
+
+
 Arguments sigTok : simpl never.
 
-Definition sigHAd := FinType (EqType sigNat).
+Definition sigHAd := sigNat.
 Arguments sigHAd : simpl never.
+Definition sigHAd_fin := FinType(EqType sigHAd).
 
-Definition sigPro := FinType (EqType (sigList sigTok)).
+Definition sigPro := sigList sigTok.
 Arguments sigPro : simpl never.
 Instance Encode_Prog : codable sigPro Pro := _.
+Definition sigPro_fin := FinType(EqType sigPro).
 
-Definition sigHClos := FinType (EqType (sigPair sigPro sigHAd)).
+Definition sigHClos := sigPair sigPro sigHAd.
 Arguments sigHClos : simpl never.
-Instance Encode_HClos : codable sigHClos HClos := _.
+Instance Encode_HClos : codable (FinType (EqType sigHClos)) HClos := _.
+Definition sigHClos_fin := FinType(EqType sigHClos).
 
-Definition sigHEnt' := FinType (EqType (sigPair sigHClos sigHAd)).
+Definition sigHEnt' := sigPair sigHClos sigHAd.
 Arguments sigHEnt' : simpl never.
-Instance Encode_HEnt' : codable sigHEnt' (HClos*HAd) := _.
+Instance Encode_HEnt' : codable (FinType (EqType sigHEnt')) (HClos*HAd) := _.
+Definition sigHEnt'_fin := FinType(EqType sigHEnt').
 
-Definition sigHEnt := FinType (EqType (sigOption sigHEnt')).
+Definition sigHEnt := sigOption sigHEnt'.
 Arguments sigHEnt : simpl never.
-Instance Encode_HEnt : codable sigHEnt HEnt := _.
+Instance Encode_HEnt : codable (FinType (EqType sigHEnt)) HEnt := _.
+Definition sigHEnt_fin := FinType(EqType sigHEnt).
 
-Definition sigHeap := FinType (EqType (sigList sigHEnt)).
+Definition sigHeap := sigList sigHEnt.
 Arguments sigHeap : simpl never.
-Instance Encode_Heap : codable sigHeap Heap := _.
+Instance Encode_Heap : codable (FinType (EqType sigHeap)) Heap := _.
+Definition sigHeap_fin := FinType(EqType sigHeap).
